stack push proof

treiber_stack.v
@@ -2,27 +2,127 @@ From iris.program_logic Require Export weakestpre.
 From iris.proofmode Require Import invariants ghost_ownership.
 From iris.heap_lang Require Export lang.
 From iris.heap_lang Require Import proofmode notation.
+From iris.algebra Require Import upred upred_big_op.
+From iris.tests Require Import atomic.
 
-Section treiber_stack.
-  Context `{!heapG Σ} (N: namespace).
+Definition new_stack: val := λ: <>, ref NONE.
 
-  Definition push_treiber: val :=
-    rec: "push_treiber" "lhd" "x" :=
-      let: "hd" := !"lhd" in
-      let: "hd'" := ("x", SOME "lhd") in
-      if: CAS "lhd" "hd" "hd'"
+Definition push: val :=
+  rec: "push" "s" "x" :=
+      let: "hd" := !"s" in
+      let: "s'" := SOME ("x", ref "hd") in
+      if: CAS "s" "hd" "s'"
         then #()
-        else "push_treiber" "lhd" "x".
+        else "push" "s" "x".
 
-  Definition pop_treiber: val :=
-    rec: "pop_treiber" "lhd" :=
-      let: "hd" := !"lhd" in
+Definition pop: val :=
+  rec: "pop" "s" :=
+      let: "hd" := !"s" in
       match: "hd" with
         SOME "pair" =>
-        if: CAS "lhd" "hd" (Snd "pair")
+        if: CAS "s" "hd" (Snd "pair")
           then SOME (Fst "pair")
-          else "pop_treiber" "lhd"
+          else "pop" "s"
       | NONE => NONE
       end.
 
-End treiber_stack.
+Section proof.
+  Context `{!heapG Σ} (N: namespace) (R: val → iProp Σ) `{∀ v, TimelessP (R v)}.
+
+  Fixpoint is_stack (s: loc) (xs: list val) : iProp Σ :=
+    match xs with
+    | [] => (s ↦ NONEV)%I
+    | x :: xs => (∃ s': loc, s ↦ SOMEV (x, #s') ★ R x ★ is_stack s' xs)%I
+    end.
+
+  Definition is_some_stack (s: loc) : iProp Σ := (∃ xs: list val, is_stack s xs)%I.
+
+  Definition stack_inv s : iProp Σ := inv N (is_some_stack s).
+
+  Instance stack_inv_persistent s: PersistentP (stack_inv s).
+  Proof. apply _. Qed.
+
+  Instance is_stack_timeless: ∀ xs s, TimelessP (is_stack s xs).
+  Proof.
+    induction xs as [|? xs'].
+    - apply _.
+    - simpl. intros s.
+      apply uPred.exist_timeless.
+      intros s'. specialize IHxs' with s'.
+      apply _.
+  Qed.
+
+  Instance is_some_stack_timeless: ∀ s, TimelessP (is_some_stack s).
+  Proof.
+    intros s. rewrite /is_some_stack. apply uPred.exist_timeless. intros ?. apply is_stack_timeless.
+  Qed.
+
+  Lemma new_stack_spec:
+    ∀ (Φ: val → iProp Σ),
+      heapN ⊥ N →
+      heap_ctx ★ (∀ s, is_stack s [] -★ Φ #s) ⊢ WP new_stack #() {{ Φ }}.
+  Proof. iIntros (Φ HN) "[#Hh HΦ]". wp_seq. wp_alloc l as "Hl". by iApply "HΦ". Qed.
+
+  Definition push_triple (s: loc) (x: val) :=
+    atomic_triple (fun xs => R x ★ is_stack s xs)%I
+                  (fun xs _ => is_stack s (x :: xs))
+                  (nclose heapN)
+                  ⊤
+                  (push #s x).
+  
+  Lemma push_atomic_spec (s: loc) (x: val) :
+    heapN ⊥ N → heap_ctx ⊢ push_triple s x.
+  Proof.
+    iIntros (HN) "#?".
+    rewrite /push_triple /atomic_triple.
+    iIntros (P Q) "#Hvs".
+    iLöb as "IH". iIntros "!# HP". wp_rec.
+    wp_let. wp_bind (! _)%E.
+    iVs ("Hvs" with "HP") as (xs) "[[Hx Hxs] [Hvs' _]]".
+    destruct xs as [|y xs'].
+    - simpl. wp_load. iVs ("Hvs'" with "[Hx Hxs]") as "HP"; first by iFrame.
+      iVsIntro. wp_let. wp_alloc l as "Hl". wp_let.
+      wp_bind (CAS _ _ _)%E.
+      iVs ("Hvs" with "HP") as (xs) "[[Hx Hxs] Hvs']".
+      destruct xs as [|y xs'].
+      + simpl. wp_cas_suc.
+        iDestruct "Hvs'" as "[_ Hvs']".
+        iVs ("Hvs'" $! #() with "[Hl Hx Hxs]") as "HQ".
+        {  iExists l. by iFrame. }
+        iVsIntro. wp_if. iVsIntro. eauto.
+      + simpl. iDestruct "Hxs" as (s') "(Hs & Hy & Hs')".
+        wp_cas_fail.
+        iDestruct "Hvs'" as "[Hvs' _]".
+        iVs ("Hvs'" with "[Hx Hs Hy Hs']").
+        { iFrame. iExists s'. by iFrame. }
+        iVsIntro. wp_if. by iApply "IH".
+    - simpl.
+      iDestruct "Hxs" as (s') "(Hs & Hy & Hs')".
+      wp_load. iVs ("Hvs'" with "[Hx Hs Hy Hs']") as "HP".
+      { iFrame. iExists s'. by iFrame. }
+      iVsIntro. wp_let. wp_alloc l as "Hl".
+      wp_let. wp_bind (CAS _ _ _)%E.
+      iVs ("Hvs" with "HP") as (xs) "[[Hx Hxs] Hvs']".
+      destruct xs as [|y' xs''].
+      + simpl. wp_cas_fail.
+        iDestruct "Hvs'" as "[Hvs' _]".
+        iVs ("Hvs'" with "[Hx Hxs]"); first by iFrame.
+        iVsIntro. wp_if. by iApply "IH".
+      + simpl. iDestruct "Hxs" as (s'') "(Hs & Hy' & Hs'')".
+        destruct (decide (s' = s'' ∧ y = y')) as [[]|Hneq].
+        * subst. wp_cas_suc.
+          iDestruct "Hvs'" as "[_ Hvs']".
+          iVs ("Hvs'" $! #() with "[Hs Hx Hl Hy' Hs'']") as "HQ".
+          { iExists l. iFrame. iExists s''. by iFrame. }
+          iVsIntro. wp_if. iVsIntro. eauto.
+        * wp_cas_fail.
+          { intros Heq. apply Hneq. by inversion Heq. }
+          iDestruct "Hvs'" as "[Hvs' _]".
+          iVs ("Hvs'" with "[Hx Hs Hy' Hs'']").
+          { iFrame. iExists s''. by iFrame. }
+          iVsIntro. wp_if. by iApply "IH".
+  Qed.
+  
+    
+End proof.
+
